Updated model

model/buffer.dfy
@@ -3,3 +3,18 @@ include "flit.dfy"
 datatype Buffer =
   | Node(dest: nat, next: Buffer)
   | None
+  {
+    predicate is_prefix_of(b: Buffer) {
+      match (this, b)
+      case (Node(dest, next), Node(dest', next')) => dest == dest' && next.is_prefix_of(next')
+      case (None, Node(_, _)) => true
+      case (None, None) => true
+      case (Node(_, _), None) => false
+    }
+
+    function length(): nat {
+      match this
+      case None => 0
+      case Node(_, next) => 1 + next.length()
+    }
+  }
