model/noc.dfy
@@ -1,0 +1,16 @@
+include "router.dfy"
+
+type Noc = seq<seq<Router>>
+
+ghost predicate Valid(n: Noc)
+{
+  && |n| >= 2
+  && (forall i :: 0 <= i < |n| ==> |n[i]| == |n|)
+  && (forall i, j :: 0 <= i < |n| && 0 <= j < |n| ==> n[i][j].id == i*|n| + j)
+}
+
+ghost predicate containsId(n: Noc, id: Id)
+  requires Valid(n)
+{
+  exists i, j :: n[i][j].id == id
+}
